02Stack/StackConversion.thy
@@ -2,8 +2,13 @@ theory StackConversion
 imports EvaluateStack
 begin
 
+primrec invert :: "nat list \<Rightarrow> nat list" where
+  "invert [] = []"
+| "invert (x # xs) = insert_at x 0 (invert xs)"
+
 abbreviation unfold_heap :: "expr heap \<Rightarrow> expr \<Rightarrow> nat list \<Rightarrow> expr" where
-  "unfold_heap h \<equiv> foldl (\<lambda>e x. Let (lookup\<^sub>h h x) (incr\<^sub>e\<^sub>e x e))"
+  "unfold_heap h e rs \<equiv> 
+    fst (foldl (\<lambda>(e, rs) x. (Let (subst\<^sub>x\<^sub>e\<^sub>s (invert rs) (lookup\<^sub>h h x)) e, tl rs)) (e, rs) rs)"
 
 fun unstack :: "nat list list \<Rightarrow> frame list \<Rightarrow> expr \<Rightarrow> expr heap \<Rightarrow> expr" where
   "unstack [] s e h = e"
@@ -21,95 +26,94 @@ fun unstack_state :: "nat list list \<Rightarrow> stack_state \<Rightarrow> expr
 | "unstack_state rs (StackState (Return v) s h) = unstack rs s (devalue v) h"
 
 abbreviation map_through :: "'a list \<Rightarrow> nat list \<Rightarrow> 'a list" where
-  "map_through \<Gamma> \<equiv> map (the o lookup \<Gamma>)"
+  "map_through \<Gamma> \<equiv> map (\<lambda>x. the (lookup \<Gamma> x))"
 
-fun safe_unfold_order' :: "nat list list \<Rightarrow> nat set \<Rightarrow> expr heap \<Rightarrow> frame list \<Rightarrow> bool" where
-  "safe_unfold_order' [] xs h s = True"
-| "safe_unfold_order' ([] # rss) xs h s = safe_unfold_order' rss xs h (tl s)"
-| "safe_unfold_order' ((r # rs) # rss) xs h s = (
-    (\<forall>x. x < length\<^sub>h h \<longrightarrow> x \<notin> xs \<longrightarrow> r \<notin> free_vars (lookup\<^sub>h h x)) \<and> (r \<notin> free_vars\<^sub>s\<^sub>s s) \<and>
-      safe_unfold_order' (rs # rss) (insert r xs) h s)"
+fun safe_unfold_order' :: "nat list list \<Rightarrow> expr heap \<Rightarrow> frame list \<Rightarrow> bool" where
+  "safe_unfold_order' [] h s = True"
+| "safe_unfold_order' ([] # rss) h s = safe_unfold_order' rss h (tl s)"
+| "safe_unfold_order' ((r # rs) # rss) h s = (
+    (free_vars (lookup\<^sub>h h r) \<subseteq> set (rs @ concat rss)) \<and> (r \<notin> free_vars\<^sub>s\<^sub>s s) \<and>
+      safe_unfold_order' (rs # rss) h s)"
 
 fun safe_unfold_order :: "nat list list \<Rightarrow> expr heap \<Rightarrow> frame list \<Rightarrow> type list \<Rightarrow> bool" where
   "safe_unfold_order rss h s \<Gamma> = (distinct (concat rss) \<and> length (concat rss) = length \<Gamma> \<and> h \<turnstile>\<^sub>h \<Gamma> \<and>
     length rss = Suc (length s) \<and> (\<forall>r \<in> set (concat rss). r < length \<Gamma>) \<and> 
-      safe_unfold_order' rss {} h s)"
+      safe_unfold_order' rss h s)"
 
-lemma [simp]: "[],map_through \<Gamma> rs \<turnstile> e : t \<Longrightarrow> distinct rs \<Longrightarrow> h \<turnstile>\<^sub>h \<Gamma> \<Longrightarrow> length rs = length \<Gamma> \<Longrightarrow> 
-  \<forall>i < length rs. rs ! i + i < length \<Gamma> \<Longrightarrow> \<forall>x < length\<^sub>h h. \<forall>r \<in> set rs. r \<notin> free_vars (lookup\<^sub>h h x) \<Longrightarrow> 
-    unfold_heap (e, h) rs = (e', h') \<Longrightarrow> [],[] \<turnstile> e' : t"
-  proof (induction rs arbitrary: \<Gamma> e h)
+lemma [simp]: "lookup \<Gamma> r = Some tt \<Longrightarrow> insert_at 0 tt (map_through \<Gamma> rs) = map_through \<Gamma> (r # rs)" 
+  by (cases "map_through \<Gamma> rs") simp_all
+
+lemma [simp]: "\<Delta>,\<Gamma> \<turnstile> e : t \<Longrightarrow> \<Delta>,map_through \<Gamma> rs \<turnstile> subst\<^sub>x\<^sub>e\<^sub>s (invert rs) e : t"
+  apply (induction rs)
+  apply simp_all
+  by simp
+
+lemma [simp]: "[],map_through \<Gamma> rs \<turnstile> e : t \<Longrightarrow> distinct rs \<Longrightarrow> 
+  \<forall>r \<in> set rs. r < length \<Gamma> \<Longrightarrow> h \<turnstile>\<^sub>h \<Gamma> \<Longrightarrow> safe_unfold_order' [rs] h [] \<Longrightarrow>
+    [],[] \<turnstile> unfold_heap h e rs : t"
+  proof (induction rs arbitrary: e)
   case Nil
-    from Nil(7) have "e' = e" by simp
-    with Nil(1) show ?case by simp
+    from Nil(1) show ?case by simp
   next case (Cons r rs)
-    from Cons(2) have "[],the (lookup \<Gamma> r) # map_through (remove \<Gamma> r) rs \<turnstile> e : t" by simp
-    from Cons(3) have "distinct (r # rs)" by simp
-    from Cons(4) have "h \<turnstile>\<^sub>h \<Gamma>" by simp
-    from Cons(5) have "Suc (length rs) = length \<Gamma>" by simp
-    from Cons(6) have R: "r < length \<Gamma>" by auto
-    from Cons(6) have "\<forall>i < Suc (length rs). (r # rs) ! i + i < length \<Gamma>" by simp
-    from Cons(7) have "\<forall>x<length\<^sub>h h. \<forall>r\<in>set (r # rs). r \<notin> free_vars (lookup\<^sub>h h x)" by simp
+    from Cons have "[],map_through \<Gamma> (r # rs) \<turnstile> e : t" by blast
+    from Cons have "distinct (r # rs)" by simp
+    from Cons have "\<forall>r\<in>set (r # rs). r < length \<Gamma>" by simp
+    then obtain tt where T: "lookup \<Gamma> r = Some tt" by fastforce
+
+    from Cons(5) have "h \<turnstile>\<^sub>h \<Gamma>" by simp
+    with T have "[],\<Gamma> \<turnstile> lookup\<^sub>h h r : tt" by (simp add: typecheck_heap_def)
+
+    from Cons have "free_vars (lookup\<^sub>h h r) \<subseteq> set rs" by simp
+    from Cons have "safe_unfold_order' [rs] h []" by simp
 
 
 
-    have X: "[],map_through (remove \<Gamma> r) rs \<turnstile> lookup\<^sub>h h r : the (lookup \<Gamma> r)" by simp
-    from Cons(2) have "[],insert_at 0 (the (lookup \<Gamma> r)) (map_through (remove \<Gamma> r) rs) \<turnstile> e : t" 
-      by (cases "map_through (remove \<Gamma> r) rs") simp_all
-    with X have A: "[],map_through (remove \<Gamma> r) rs \<turnstile> Let (lookup\<^sub>h h r) e : t" by simp
+    have "[],map_through \<Gamma> rs \<turnstile> subst\<^sub>x\<^sub>e\<^sub>s (invert (r # rs)) (lookup\<^sub>h h r) : tt" by simp
+    moreover from Cons(2) T have "[],insert_at 0 tt (map_through \<Gamma> rs) \<turnstile> e : t" by simp
+    ultimately have A: "[],map_through \<Gamma> rs \<turnstile> Let (subst\<^sub>x\<^sub>e\<^sub>s (invert (r # rs)) (lookup\<^sub>h h r)) e : t" by simp
     from Cons have B: "distinct rs" by simp
-    from Cons(4, 7) R have C: "map\<^sub>h (decr\<^sub>x\<^sub>e r) (remove\<^sub>h h r) \<turnstile>\<^sub>h remove \<Gamma> r" by simp
-    from Cons(5) R have D: "length rs = length (remove \<Gamma> r)" by simp
-    from Cons(6) R have E: "\<forall>i<length rs. rs ! i + i < length (remove \<Gamma> r)" by auto
-
-
-    have F: "\<forall>x<length\<^sub>h (map\<^sub>h (decr\<^sub>x\<^sub>e r) (remove\<^sub>h h r)). \<forall>rr\<in>set rs. 
-        rr \<notin> free_vars (lookup\<^sub>h (map\<^sub>h (decr\<^sub>x\<^sub>e r) (remove\<^sub>h h r)) x)" 
-      proof (rule, rule, rule)
-        fix x rr
-        assume X: "x < length\<^sub>h (map\<^sub>h (decr\<^sub>x\<^sub>e r) (remove\<^sub>h h r))"
-
-
-        assume RS: "rr \<in> set rs"
-
-
-        from R Cons(4) have R': "r < length\<^sub>h h" by auto
-
-
-        from X R' have "incr r x < length\<^sub>h h" by (auto simp add: incr_def)
-        with Cons(7) have Y: "r \<notin> free_vars (lookup\<^sub>h h (incr r x))" by simp
-
-
-
-        have "incr r rr \<notin> free_vars (lookup\<^sub>h h (incr r x))" by simp
-        with R' Y show "rr \<notin> free_vars (lookup\<^sub>h (map\<^sub>h (decr\<^sub>x\<^sub>e r) (remove\<^sub>h h r)) x)" by simp
-      qed
-    from Cons have "unfold_heap (Let (lookup\<^sub>h h r) e, map\<^sub>h (decr\<^sub>x\<^sub>e r) (remove\<^sub>h h r)) rs = (e', h')"
-      by simp
-    with Cons(1) A B C D E F show ?case by blast
+    from Cons have C: "\<forall>r\<in>set rs. r < length \<Gamma>" by simp
+    from Cons have D: "h \<turnstile>\<^sub>h \<Gamma>" by simp
+    from Cons have "safe_unfold_order' [rs] h []" by simp
+    with Cons(1) A B C D have 
+      "[],[] \<turnstile> unfold_heap h (Let (subst\<^sub>x\<^sub>e\<^sub>s (invert (r # rs)) (lookup\<^sub>h h r)) e) rs : t" by blast
+    thus ?case by simp
   qed
 
 lemma tc_unstack [elim]: "map_through \<Gamma> (concat rs) \<turnstile>\<^sub>s\<^sub>s s : t \<rightarrow> t' \<Longrightarrow> 
-  [],map_through \<Gamma> (concat rs) \<turnstile> e : t \<Longrightarrow> safe_unfold_order rs h s \<Gamma> \<Longrightarrow> 
-    unstack rs s (e, h) = (e', h') \<Longrightarrow> [],[] \<turnstile> e' : t'"
-  proof (induction rs s "(e, h)" arbitrary: \<Gamma> rule: unstack.induct)
+  \<Delta>,map_through \<Gamma> (concat rs) \<turnstile> e : t \<Longrightarrow> safe_unfold_order rs h s \<Gamma> \<Longrightarrow> 
+    \<Delta>,[] \<turnstile> unstack rs s e h : t'"
+  proof (induction rs s e h rule: unstack.induct)
   case 1
     thus ?case by auto
-  next case (2 rs rss \<Gamma>)
+  next case (2 rs rss e h)
     hence T: "t = t'" by auto
-    moreover from 2 have "[],[] \<turnstile> e' : t" by fastforce
-    ultimately show ?case by simp
-  next case (3 r rs x s eh)
+
+
+    from 2 have "distinct rs" by auto
+    from 2 have "length rs = length \<Gamma>" by auto
+    from 2 have "h \<turnstile>\<^sub>h \<Gamma>" by auto
+    from 2 have RSS: "rss = []" by auto
+    from 2 have "\<forall>r \<in> set rs. r < length \<Gamma>" by auto
+    from 2 have "safe_unfold_order' [rs] h []" by auto
+
+
+    from 2(3) RSS have "\<Delta>,map_through \<Gamma> rs \<turnstile> e : t" by (metis concat.simps append_Nil2)
+
+
+    hence "\<Delta>,[] \<turnstile> unfold_heap h e rs : t" by simp
+    with T RSS show ?case by simp
+  next case (3 r rs x s e h)
     thus ?case by simp
-  next case (4 r rs e\<^sub>2 s eh)
+  next case (4 r rs e\<^sub>2 s e h)
     thus ?case by simp
-  next case (5 r rs l s eh)
+  next case (5 r rs l s e h)
     thus ?case by simp
-  next case (6 r rs t cs s eh)
+  next case (6 r rs t cs s e h)
     thus ?case by simp
-  next case (7 r rs t s eh)
+  next case (7 r rs t s e h)
     thus ?case by simp
-  next case (8 r rs t s eh)
+  next case (8 r rs t s e h)
     thus ?case by simp
   qed
 
